Format Spec. Avoid using trivial refine in proof.

Paxos/Spec.lean
@@ -1,6 +1,6 @@
 /- Basic Paxos specification, translated from the spec in TLA+
    in https://arxiv.org/pdf/1802.09687, Appendix A, by Chand and Liu, referred to as CL.
-  --! indicates the differences of this spec from the spec in CL
+  ! indicates the differences of this spec from the spec in CL
 -/
 import Mathlib.Tactic
 
@@ -22,19 +22,21 @@ abbrev Ballot := Nat
 -/
 instance : HAdd (Option Ballot) Nat (Option Ballot) where
   hAdd
-    | none,    0          => none         -- -1 + 0     = -1
-    | none,    Nat.succ k => k            -- 0  + (k+1) = k
-    | some a,  b          => a + b        -- a  +  b    = a + b
+  | none,    0          => none         -- -1 + 0     = -1
+  | none,    Nat.succ k => k            -- 0  + (k+1) = k
+  | some a,  b          => a + b        -- a  +  b    = a + b
 
-/-- Message is defined as an inductive type -/
---! in oneb `maxVBal` and `maxVal` are defined to be `Option` type.
---! in twob `bal` and `val` are also defined to be `Option` type. This is to ensure type
---!   compatibility with `max_prop`.
+/-- Message is defined as an inductive type
+  ! In oneb `maxVBal` and `maxVal` are defined to be `Option` type.
+  ! In twob `bal` and `val` are also defined to be `Option` type. The option type are only
+  used in `max_prop`, to ensure type compatibility when `twobs` is empty. In Phase 2b, they
+  can't be `none` as we only send valid ballots and values.
+-/
 inductive Message where
-  | onea  (bal : Ballot)
-  | oneb  (bal : Ballot) (maxVBal : Option Ballot) (maxVal : Option Value) (acc : Acceptor)
-  | twoa  (bal : Ballot) (val : Value)
-  | twob  (bal : Option Ballot) (val : Option Value) (acc : Acceptor)
+  | onea (bal : Ballot)
+  | oneb (bal : Ballot) (maxVBal : Option Ballot) (maxVal : Option Value) (acc : Acceptor)
+  | twoa (bal : Ballot) (val : Value)
+  | twob (bal : Option Ballot) (val : Option Value) (acc : Acceptor)
 
 /- Quorums and QuorumAssumption. Same as in TLA. -/
 
@@ -54,35 +56,32 @@ def Phase1a (b : Ballot) : Prop :=
   sent' = Send (Message.onea b) sent
 
 /-- Get the maximum ballot and value that an acceptor has voted for.
---! In TLA, when `twobs` is empty it returns a record with `bal` and `val` begin set to
---!  False. Otherwise, it returns a set of `2b` messages. Here we always return a set
---!  of `2b` messages to ensure the type compatibility.
+  ! In TLA, when `twobs` is empty it returns a record with `bal` and `val` begin set to
+  False. Otherwise, it returns a set of `2b` messages. Here we always return a set of `2b`
+  messages to ensure the type compatibility.
 -/
 def max_prop (a : Acceptor): Set Message :=
   let twobs := {m ∈ sent | ∃ (b: Ballot) (v: Value), m = Message.twob b v a}
   if twobs ≠ ∅ then
-      {m₁ ∈ twobs | ∀m₂ ∈ twobs, ∃ (b₁ b₂: Ballot) (v₁ v₂: Value),
-                      m₁ = Message.twob b₁ v₁ a ∧ m₂ = Message.twob b₂ v₂ a ∧ b₁ ≥ b₂}
+      {m₁ ∈ twobs | ∀ m₂ ∈ twobs, ∃ (b₁ b₂: Ballot) (v₁ v₂: Value),
+                        m₁ = Message.twob b₁ v₁ a
+                      ∧ m₂ = Message.twob b₂ v₂ a
+                      ∧ b₁ ≥ b₂}
   else {Message.twob none none a}  -- return `none` for both `maxVBal` and `maxVal`.
 
-/-- Phase1b. Same as in TLA except using pattern matching and conditional (`if-else`).
---! Need the conditional to say when the guard is not satisfied: `sent' = sent`.
--/
+/-- Phase1b. Same as in TLA except using pattern matching. -/
 def Phase1b (a : Acceptor) : Prop :=
-  ∃ m ∈ sent, ∃r ∈ max_prop sent a,
+  ∃ m ∈ sent, ∃ r ∈ max_prop sent a,
     match m, r with
-    | Message.onea b, Message.twob rbal rval _a =>
-        (∀m2 ∈ sent, match m2 with
-                      | Message.oneb b2 _ _ a' => (a' = a) → (b > b2)
-                      | Message.twob b2 _ a' => (a' = a) → (b > b2)
-                      | _ => True)
+    | Message.onea b, Message.twob rbal rval _ =>
+        (∀ m₂ ∈ sent, match m₂ with
+                      | Message.oneb b₂ _ _ a' => a' = a → b > b₂
+                      | Message.twob b₂ _ a'   => a' = a → b > b₂
+                      | _                      => True)
         ∧ sent' = Send (Message.oneb b rbal rval a) sent
     | _, _ => False
 
-/-- Phase 2a. Same as in TLA except using pattern matching and conditional (`if-else`).
---- We also have nested `if-else` in Phase2a because in the second one we need
-     `Classical.choose` to pick `v` from the existential statement.
--/
+/-- Phase 2a. Same as in TLA except using pattern matching. -/
 def Phase2a (b : Ballot) : Prop :=
   (¬∃ m ∈ sent, match m with
                 | Message.twoa b' _ => b' = b
@@ -113,22 +112,22 @@ def Phase2b (a : Acceptor) : Prop :=
                   ∧ sent' = Send (Message.twob b v a) sent
               | _ => False
 
-/-- Init. Same as in TLA. -/
+/-- Initial state, asserts `sent = ∅`. Same as in TLA. -/
 def Init : Prop := sent = ∅
 
-/-- Next. Same as in TLA. -/
+/-- State transition. Same as in TLA. -/
 def Next : Prop :=    (∃b, Phase1a sent sent' b ∨ Phase2a Quorums sent sent' b)
                     ∨ (∃a, Phase1b sent sent' a ∨ Phase2b sent sent' a)
 
 /--
     This is `Spec == Init /\ [][Next]_vars` in TLA+.
-    --! We model the temporal logic formula using trace.
-    --! named `PaxosSpec` to avoid name clashes with the `Spec` namespace.
+  ! We model the temporal logic formula using trace.
+  ! It is named `PaxosSpec` to avoid name clashes with the `Spec` namespace.
     `σ` represents the trace of the system, which is mapping from `ℕ` to `Set Message`.
       1. The initial state is `Init (σ 0)`
       2. The next state is defined by the relation (allowing stuttering)
          `Next Quorums (σ i) (σ (i+1)) ∨ (σ i) = (σ (i+1))`.
-    For trace, also see (Igor Konnov):
+    For trace, also see this post by Igor Konnov:
       https://protocols-made-fun.com/lean/2025/06/10/lean-epfd-completeness.html
 -/
 def PaxosSpec (σ : ℕ → Set Message) : Prop :=
